GVN.v
@@ -118,8 +118,14 @@ Proof.
     unfold Ir.SmallStep.gep in H1.
     destruct p2.
     { destruct inb.
-      { des_ifs.
-        eexists. eexists . reflexivity. }
+      { destruct (Ir.Memory.get m b) eqn:HGET.
+        destruct (Ir.MemBlock.inbounds n t0 &&
+         Ir.MemBlock.inbounds
+           (Ir.SmallStep.twos_compl_add n (idx * Ir.ty_bytesz t) Ir.MEMSZ) t0)
+                 eqn:HINB.
+        eexists. eexists. reflexivity.
+        eexists. eexists. reflexivity.
+        eexists. eexists. reflexivity. }
       { eexists. eexists . reflexivity. }
     }
     { destruct inb.
@@ -127,6 +133,26 @@ Proof.
       { congruence. }
     }
   }
+Qed.
+
+Lemma ir_ptr_pphy_inj:
+  forall o1 I1 cid1 o2 I2 cid2
+         (H:Ir.ptr (Ir.pphy o1 I1 cid1) = Ir.ptr (Ir.pphy o2 I2 cid2)),
+    o1 = o2 /\ I1 = I2 /\ cid1 = cid2.
+Proof.
+  intros.
+  inv H.
+  split. reflexivity. split. reflexivity. reflexivity.
+Qed.
+
+Lemma ir_ptr_plog_inj:
+  forall l1 o1 l2 o2
+         (H:Ir.ptr (Ir.plog l1 o1) = Ir.ptr (Ir.plog l2 o2)),
+    l1 = l2 /\ o1 = o2.
+Proof.
+  intros.
+  inv H.
+  split. reflexivity. split.
 Qed.
 
 Lemma physicalized_ptr_phy:
@@ -162,38 +188,87 @@ Proof.
       exfalso. apply HPP. eexists. eexists. reflexivity.
     }
     { unfold Ir.SmallStep.gep in HP1'.
-      des_ifs.
+      
+      destruct p1 eqn:HP;
+      destruct inb eqn:HINB.
+      destruct (Ir.Memory.get m b) eqn:HGET.
+      destruct (Ir.MemBlock.inbounds n0 t0 &&
+           Ir.MemBlock.inbounds
+             (Ir.SmallStep.twos_compl_add n0 (idx * Ir.ty_bytesz t) Ir.PTRSZ) t0)
+               eqn:HINB2.
+      ss.
+      ss.
+      ss.
+      congruence.
+      destruct (idx * Ir.ty_bytesz t <? Nat.shiftl 1 (Ir.PTRSZ - 1)) eqn:HSHL.
       {
-        exploit IHHPP.
-        { reflexivity. }
-        { reflexivity. }
-        intros HH.
-        unfold Ir.SmallStep.gep in HP2'.
-        des_ifs.
-        { inv HH. destruct H0.
-          split. reflexivity.
-          split. constructor. constructor. assumption.
-          assumption.
+        destruct (n0 + idx * Ir.ty_bytesz t <? Ir.MEMSZ) eqn:HOFS.
+        {
+          apply ir_ptr_pphy_inj in HP1'.
+          destruct HP1'. destruct H0.
+          exploit IHHPP.
+          { reflexivity. }
+          { reflexivity. }
+          intros HH. destruct HH. destruct H3.
+          unfold Ir.SmallStep.gep in HP2'.
+          rewrite HSHL in HP2'.
+          destruct (n + idx * Ir.ty_bytesz t <? Ir.MEMSZ) eqn:HN.
+          { apply ir_ptr_pphy_inj in HP2'. destruct HP2'.
+            split.
+            { congruence. }
+            split.
+            { rewrite H0.
+              destruct H6. rewrite H6.
+              rewrite H2. constructor. constructor. assumption. }
+            { destruct H6. congruence. }
+          }
+          { ss. }
         }
+        { ss. }
       }
       { exploit IHHPP; try reflexivity.
         intros HH.
         inv HH. destruct H0.
         unfold Ir.SmallStep.gep in HP2'.
-        des_ifs.
-        split. reflexivity.
-        split. constructor. constructor. assumption.
-        reflexivity.
+        apply ir_ptr_pphy_inj in HP1'.
+        destruct HP1'. destruct H2.
+        rewrite HSHL in HP2'.
+        apply ir_ptr_pphy_inj in HP2'.
+        destruct HP2'. destruct H5.
+        split. congruence.
+        split. rewrite H2, H5. constructor. constructor. assumption.
+        congruence.
       }
       { exploit IHHPP; try reflexivity.
         intros HH.
         inv HH. destruct H0.
         unfold Ir.SmallStep.gep in HP2'.
-        des_ifs.
+        apply ir_ptr_pphy_inj in HP2'.
+        destruct HP2'. destruct H2.
+        apply ir_ptr_pphy_inj in HP1'.
+        destruct HP1'. destruct H5.
+        split. congruence. split. congruence. congruence.
       }
     }
   }
 Qed.
+
+Lemma PTRSZ_MEMSZ:
+  Nat.shiftl 2 (Ir.PTRSZ - 1) = Ir.MEMSZ.
+Proof. reflexivity. Qed.
+
+Lemma MEMSZ_nonzero:
+Ir.MEMSZ <> 0.
+Proof.
+  unfold Ir.MEMSZ.
+  unfold Ir.PTRSZ.
+  intros HH. simpl in HH.
+  repeat (rewrite Nat.double_twice in HH).
+  omega.
+Qed.
+
+Opaque Ir.PTRSZ.
+Opaque Ir.MEMSZ.
 
 Lemma physicalized_ptr_log:
   forall m l1 o1 o2 Is2 cid2 v1 v2 mb
@@ -209,6 +284,7 @@ Proof.
   generalize dependent o2.
   generalize dependent Is2.
   generalize dependent cid2.
+  generalize dependent mb.
   induction HPP.
   { intros.
     inv HV1.
@@ -228,46 +304,883 @@ Proof.
       exfalso. apply HPP. eexists. eexists. reflexivity.
     }
     { unfold Ir.SmallStep.gep in HP1'.
-      des_ifs.
-      {
-        exploit IHHPP.
-        { reflexivity. }
-        { reflexivity. }
-        { assumption. }
-        intros HH.
-        unfold Ir.SmallStep.gep in HP2'.
-        destruct ((idx * N.of_nat (Ir.ty_bytesz t) <?
-            N.shiftl 1 (N.of_nat Ir.PTRSZ - 1))%N) eqn:H11.
-        { (* positive offset add *)
-          destruct (N.to_nat
-             (Ir.SmallStep.twos_compl_add (N.of_nat n)
-                (idx * N.of_nat (Ir.ty_bytesz t)) Ir.PTRSZ) <? Ir.MEMSZ) eqn:H2.
-          { assert 
-        des_ifs.
-        { inv HH. destruct H0.
-          split. reflexivity.
-          split. constructor. constructor. assumption.
-          assumption.
+      destruct p1 eqn:HP.
+      { (* log *)
+        destruct inb eqn:HINB.
+        { (* inbounds *)
+          destruct (Ir.Memory.get m b) eqn:HGETB; try ss.
+          exploit IHHPP.
+          { reflexivity. }
+          { reflexivity. }
+          { rewrite HGETB. reflexivity. }
+          intros HH.
+          unfold Ir.SmallStep.gep in HP2'.
+          destruct ((idx * (Ir.ty_bytesz t) <?
+                     Nat.shiftl 1 (Ir.PTRSZ - 1))) eqn:H11.
+          { (* positive offset add *)
+            destruct (n + idx * Ir.ty_bytesz t <? Ir.MEMSZ) eqn:H2; try congruence.
+            apply ir_ptr_pphy_inj in HP2'.
+            destruct HP2'. destruct H0.
+            rewrite PeanoNat.Nat.ltb_lt in H2.
+            destruct (Ir.MemBlock.inbounds n0 t0 &&
+                                           Ir.MemBlock.inbounds
+             (Ir.SmallStep.twos_compl_add n0 (idx * Ir.ty_bytesz t) Ir.PTRSZ) t0)
+                     eqn:HINB2.
+            { apply ir_ptr_plog_inj in HP1'. destruct HP1'. subst l1.
+              subst o1. subst o2.
+              unfold Ir.SmallStep.twos_compl_add.
+              unfold Ir.SmallStep.twos_compl.
+              rewrite PTRSZ_MEMSZ.
+              rewrite Nat.add_mod_idemp_r.
+              rewrite <- HH.
+              rewrite Nat.add_mod_idemp_l.
+              rewrite PeanoNat.Nat.add_assoc.
+              rewrite HGETB in HGET. inv HGET. reflexivity.
+              apply MEMSZ_nonzero. apply MEMSZ_nonzero.
+            }
+            { ss. }
+          }
+        { (* negaitve offset add *)
+          destruct (Ir.MemBlock.inbounds n0 t0 &&
+           Ir.MemBlock.inbounds
+             (Ir.SmallStep.twos_compl_add n0 (idx * Ir.ty_bytesz t) Ir.PTRSZ) t0)
+                   eqn:HINB2.
+          {
+            inv HP2'.
+            inv HP1'.
+            rewrite HGETB in HGET. inv HGET.
+            unfold Ir.SmallStep.twos_compl_add.
+            unfold Ir.SmallStep.twos_compl.
+            rewrite PTRSZ_MEMSZ.
+            rewrite Nat.add_mod_idemp_r.
+            rewrite Nat.add_mod_idemp_l.
+            rewrite PeanoNat.Nat.add_assoc. reflexivity.
+            apply MEMSZ_nonzero. apply MEMSZ_nonzero.
+          }
+          { ss. }
         }
       }
-      { exploit IHHPP; try reflexivity.
-        intros HH.
-        inv HH. destruct H0.
+      { (* no inbounds *)
         unfold Ir.SmallStep.gep in HP2'.
-        des_ifs.
-        split. reflexivity.
-        split. constructor. constructor. assumption.
-        reflexivity.
+        inv HP2'.
+        inv HP1'.
+        exploit IHHPP;try reflexivity; try eassumption.
+        intros HH. rewrite <- HH.
+        unfold Ir.SmallStep.twos_compl_add.
+        unfold Ir.SmallStep.twos_compl.
+        rewrite PTRSZ_MEMSZ.
+        rewrite Nat.add_mod_idemp_r.
+        rewrite Nat.add_mod_idemp_l.
+        rewrite PeanoNat.Nat.add_assoc. reflexivity.
+        apply MEMSZ_nonzero. apply MEMSZ_nonzero.
       }
-      { exploit IHHPP; try reflexivity.
-        intros HH.
-        inv HH. destruct H0.
-        unfold Ir.SmallStep.gep in HP2'.
-        des_ifs.
-      }
+    }
+    { des_ifs. }
     }
   }
 Qed.
+
+Lemma and_implies:
+  forall (P Q:Prop),
+ (P /\ (P -> Q)) -> P /\ Q.
+Proof.
+  intros.
+  destruct H.
+  split. assumption. apply H0. apply H.
+Qed.
+
+Lemma inbounds_added_abs_true:
+  forall m b t0 n0 n ofs
+    (wf_m:Ir.Memory.wf m)
+    (HGET:Ir.Memory.get m b = Some t0)
+    (HPP:(Ir.MemBlock.addr t0 + n0) mod Ir.MEMSZ = n)
+    (HINB:Ir.MemBlock.inbounds
+         (Ir.SmallStep.twos_compl_add n0 ofs Ir.PTRSZ) t0 = true),
+  Ir.MemBlock.inbounds_abs
+                      ((n + ofs) mod Ir.MEMSZ) t0 = true.
+Proof.
+  intros.
+  erewrite Ir.MemBlock.inbounds_inbounds_abs in HINB; try reflexivity.
+  rewrite <- HPP.
+  assert ((Ir.SmallStep.twos_compl_add n0 ofs Ir.PTRSZ
+           + Ir.MemBlock.addr t0) =
+          ((Ir.MemBlock.addr t0 + n0) mod Ir.MEMSZ + ofs)
+            mod Ir.MEMSZ).
+  { unfold Ir.SmallStep.twos_compl_add.
+    unfold Ir.SmallStep.twos_compl.
+    rewrite PTRSZ_MEMSZ.
+    rewrite Nat.add_mod_idemp_l.
+    rewrite Nat.add_comm.
+    rewrite <- Nat.add_assoc with (n := Ir.MemBlock.addr t0).
+    rewrite <- Nat.add_mod_idemp_r with (b := (n0 + ofs)).
+    rewrite Nat.mod_small with
+        (a := (Ir.MemBlock.addr t0 + (n0 + ofs)
+                                       mod Ir.MEMSZ)).
+    reflexivity.
+    { (* Ir.MemBlock.addr t0 + (n0 + idx * Ir.ty_bytesz t)
+         mod Ir.MEMSZ < Ir.MEMSZ *)
+      unfold Ir.MemBlock.inbounds_abs in HINB.
+      unfold in_range in HINB.
+      rewrite andb_true_iff in HINB.
+      destruct HINB.
+      rewrite PeanoNat.Nat.leb_le in H0, H.
+      unfold Ir.SmallStep.twos_compl_add in H0.
+      unfold Ir.SmallStep.twos_compl in H0.
+      rewrite PTRSZ_MEMSZ in H0.
+      rewrite Nat.add_comm with (m := Ir.MemBlock.addr t0) in H0.
+      assert (fst (Ir.MemBlock.P0_range t0) + snd (Ir.MemBlock.P0_range t0)
+              < Ir.MEMSZ).
+      { unfold Ir.MemBlock.P0_range.
+        simpl.
+        destruct wf_m.
+        symmetry in HGET.
+        eapply Ir.Memory.get_In in HGET;try reflexivity.
+        apply wf_blocks in HGET.
+        destruct HGET.
+        apply wf_inmem.
+        unfold Ir.MemBlock.addr.
+        destruct (Ir.MemBlock.P t0).
+        { simpl in wf_twin. unfold Ir.TWINCNT in wf_twin. congruence. }
+        { simpl. left. reflexivity. }
+      }
+      eapply Nat.le_lt_trans.
+      eapply H0.
+      eassumption.
+    }
+    apply MEMSZ_nonzero.
+    apply MEMSZ_nonzero.
+  }
+  rewrite H in HINB.
+  assumption.
+Qed.
+
+Lemma inbounds_abs_true:
+  forall m b t0 n0 n
+    (wf_m:Ir.Memory.wf m)
+    (HGET:Ir.Memory.get m b = Some t0)
+    (HPP:(Ir.MemBlock.addr t0 + n0) mod Ir.MEMSZ = n)
+    (HINB:Ir.MemBlock.inbounds n0 t0 = true),
+  Ir.MemBlock.inbounds_abs n t0 = true.
+Proof.
+  intros.
+  erewrite Ir.MemBlock.inbounds_inbounds_abs in HINB;
+    try reflexivity.
+  rewrite <- HPP.
+  assert ((Ir.MemBlock.addr t0 + n0) mod Ir.MEMSZ =
+          n0 + Ir.MemBlock.addr t0).
+  { unfold Ir.MemBlock.inbounds_abs in HINB.
+    unfold in_range in HINB.
+    rewrite andb_true_iff in HINB.
+    destruct HINB.
+    rewrite Nat.leb_le in H0.
+    unfold Ir.MemBlock.P0_range in H0.
+    simpl in H0.
+    inv wf_m.
+    symmetry in HGET.
+    eapply Ir.Memory.get_In in HGET; try reflexivity.
+    apply wf_blocks in HGET.
+    inv HGET.
+    rewrite Nat.mod_small.
+    omega.
+    eapply Nat.le_lt_trans.
+    rewrite Nat.add_comm.
+    eassumption.
+    eapply wf_inmem.
+    unfold Ir.MemBlock.addr.
+    destruct (Ir.MemBlock.P t0).
+    { simpl in wf_twin. unfold Ir.TWINCNT in wf_twin. omega. }
+    { simpl. eauto. }
+  }
+  rewrite H. assumption.
+Qed.
+
+Lemma inbounds_added_abs_true2:
+  forall m b t0 n0 n ofs sz
+    (wf_m:Ir.Memory.wf m)
+    (HGET:Ir.Memory.get m b = Some t0)
+    (HPP:(Ir.MemBlock.addr t0 + n0) mod Ir.MEMSZ = n)
+    (HINB:Ir.MemBlock.inbounds
+         (Ir.SmallStep.twos_compl_add n0 ofs Ir.PTRSZ + sz) t0 = true),
+  Ir.MemBlock.inbounds_abs
+                      ((n + ofs) mod Ir.MEMSZ + sz) t0 = true.
+Proof.
+  intros.
+  erewrite Ir.MemBlock.inbounds_inbounds_abs in HINB; try reflexivity.
+  rewrite <- HPP.
+  assert ((Ir.SmallStep.twos_compl_add n0 ofs Ir.PTRSZ
+           + Ir.MemBlock.addr t0) =
+          ((Ir.MemBlock.addr t0 + n0) mod Ir.MEMSZ + ofs)
+            mod Ir.MEMSZ).
+  { unfold Ir.SmallStep.twos_compl_add.
+    unfold Ir.SmallStep.twos_compl.
+    rewrite PTRSZ_MEMSZ.
+    rewrite Nat.add_mod_idemp_l.
+    rewrite Nat.add_comm.
+    rewrite <- Nat.add_assoc with (n := Ir.MemBlock.addr t0).
+    rewrite <- Nat.add_mod_idemp_r with (b := (n0 + ofs)).
+    rewrite Nat.mod_small with
+        (a := (Ir.MemBlock.addr t0 + (n0 + ofs)
+                                       mod Ir.MEMSZ)).
+    reflexivity.
+    { (* Ir.MemBlock.addr t0 + (n0 + idx * Ir.ty_bytesz t)
+         mod Ir.MEMSZ < Ir.MEMSZ *)
+      unfold Ir.MemBlock.inbounds_abs in HINB.
+      unfold in_range in HINB.
+      rewrite andb_true_iff in HINB.
+      destruct HINB.
+      rewrite PeanoNat.Nat.leb_le in H0, H.
+      unfold Ir.SmallStep.twos_compl_add in H0.
+      unfold Ir.SmallStep.twos_compl in H0.
+      rewrite PTRSZ_MEMSZ in H0.
+      rewrite Nat.add_comm with (m := Ir.MemBlock.addr t0) in H0.
+      assert (fst (Ir.MemBlock.P0_range t0) + snd (Ir.MemBlock.P0_range t0)
+              < Ir.MEMSZ).
+      { unfold Ir.MemBlock.P0_range.
+        simpl.
+        destruct wf_m.
+        symmetry in HGET.
+        eapply Ir.Memory.get_In in HGET;try reflexivity.
+        apply wf_blocks in HGET.
+        destruct HGET.
+        apply wf_inmem.
+        unfold Ir.MemBlock.addr.
+        destruct (Ir.MemBlock.P t0).
+        { simpl in wf_twin. unfold Ir.TWINCNT in wf_twin. congruence. }
+        { simpl. left. reflexivity. }
+      }
+      eapply Nat.le_lt_trans.
+      eapply Nat.le_trans with (m := Ir.MemBlock.addr t0 + ((n0 + ofs) mod Ir.MEMSZ + sz)).
+      omega.
+      eapply H0.
+      eassumption.
+    }
+    apply MEMSZ_nonzero.
+    apply MEMSZ_nonzero.
+  }
+  rewrite <- Nat.add_assoc in HINB.
+  rewrite Nat.add_comm with (n := sz) in HINB.
+  rewrite Nat.add_assoc in HINB.
+  rewrite H in HINB.
+  assumption.
+Qed.
+
+Lemma inbounds_abs_true2:
+  forall m b t0 n0 n sz
+    (wf_m:Ir.Memory.wf m)
+    (HGET:Ir.Memory.get m b = Some t0)
+    (HPP:(Ir.MemBlock.addr t0 + n0) mod Ir.MEMSZ = n)
+    (HINB:Ir.MemBlock.inbounds (n0 + sz) t0 = true),
+  Ir.MemBlock.inbounds_abs (n + sz) t0 = true.
+Proof.
+  intros.
+  erewrite Ir.MemBlock.inbounds_inbounds_abs in HINB;
+    try reflexivity.
+  rewrite <- HPP.
+  assert ((Ir.MemBlock.addr t0 + n0) mod Ir.MEMSZ =
+          n0 + Ir.MemBlock.addr t0).
+  { unfold Ir.MemBlock.inbounds_abs in HINB.
+    unfold in_range in HINB.
+    rewrite andb_true_iff in HINB.
+    destruct HINB.
+    rewrite Nat.leb_le in H0.
+    unfold Ir.MemBlock.P0_range in H0.
+    simpl in H0.
+    inv wf_m.
+    symmetry in HGET.
+    eapply Ir.Memory.get_In in HGET; try reflexivity.
+    apply wf_blocks in HGET.
+    inv HGET.
+    rewrite Nat.mod_small.
+    omega.
+    eapply Nat.le_lt_trans.
+    rewrite Nat.add_comm.
+    eapply Nat.le_trans with (m := n0 + sz + Ir.MemBlock.addr t0).
+    omega.
+    eassumption.
+    eapply wf_inmem.
+    unfold Ir.MemBlock.addr.
+    destruct (Ir.MemBlock.P t0).
+    { simpl in wf_twin. unfold Ir.TWINCNT in wf_twin. omega. }
+    { simpl. eauto. }
+  }
+  rewrite H.
+  rewrite <- Nat.add_assoc.
+  rewrite Nat.add_comm with (m := sz).
+  rewrite Nat.add_assoc.
+  assumption.
+Qed.
+
+Lemma inbounds_tcadd_abs:
+  forall m b t0 ofs n n0
+    (wf_m:Ir.Memory.wf m)
+    (HGET:Ir.Memory.get m b = Some t0)
+    (HINB:Ir.MemBlock.inbounds
+            (Ir.SmallStep.twos_compl_add n ofs Ir.PTRSZ) t0 = true)
+    (HPP:(Ir.MemBlock.addr t0 + n) mod Ir.MEMSZ = n0),
+  Ir.MemBlock.inbounds_abs
+      (Ir.SmallStep.twos_compl_add n0 ofs Ir.PTRSZ) t0 = true.
+Proof.
+  intros.
+  unfold Ir.SmallStep.twos_compl_add.
+  unfold Ir.SmallStep.twos_compl.
+  eapply inbounds_added_abs_true; try eassumption.
+Qed.
+
+Lemma list_find_key_spec {X:Type}:
+  forall (l:list (nat * X)) key val
+         (HIN:List.In (key,val) l)
+         (HNODUP:List.NoDup (list_keys l)),
+    list_find_key l key = [(key, val)].
+Proof.
+  intros.
+  remember (list_find_key l key) as res.
+  dup Heqres.
+  eapply list_find_key_NoDup in Heqres; try assumption.
+  assert (List.In (key, val) res).
+  { rewrite Heqres0.
+    eapply list_find_key_In.
+    assumption. }
+  destruct res. inv H.
+  destruct res. inv H. reflexivity. inv H0. simpl in Heqres.
+  omega.
+Qed.
+
+Lemma In_get:
+  forall m b t
+         (HWF:Ir.Memory.wf m)
+         (HIN:List.In (b, t) (Ir.Memory.blocks m)),
+    Some t = Ir.Memory.get m b.
+Proof.
+  intros.
+  unfold Ir.Memory.get.
+  assert (list_find_key (Ir.Memory.blocks m) b = [(b, t)]).
+  { eapply list_find_key_spec.
+    assumption.
+    inv HWF. assumption. }
+  rewrite H. reflexivity.
+Qed.
+
+Lemma inbounds_abs_lt_MEMSZ:
+  forall mb i
+         (HWF:Ir.MemBlock.wf mb)
+         (HINB:Ir.MemBlock.inbounds_abs i mb = true),
+    i < Ir.MEMSZ.
+Proof.
+  intros.
+  unfold Ir.MemBlock.inbounds_abs in HINB.
+  unfold in_range in HINB.
+  rewrite andb_true_iff in HINB.
+  destruct HINB.
+  rewrite PeanoNat.Nat.leb_le in H0.
+  unfold Ir.MemBlock.P0_range in *.
+  simpl in *.
+  destruct HWF.
+  eapply le_lt_trans.
+  eassumption.
+  apply wf_inmem.
+  unfold Ir.MemBlock.addr.
+  destruct (Ir.MemBlock.P mb).
+  simpl in wf_twin. unfold Ir.TWINCNT in wf_twin. congruence.
+  simpl. left. reflexivity.
+Qed.
+
+Lemma inbounds_blocks2_intersect:
+  forall m l i1 i2 I I' l'
+         (HWF:Ir.Memory.wf m)
+         (HDIFF:i1 <> i2)
+         (HINB1:Ir.Memory.inbounds_blocks2 m (i1::i2::I) = l)
+         (HINB2:Ir.Memory.inbounds_blocks2 m (i1::i2::I') = l'),
+    l = l' \/ l = [] \/ l' = [].
+Proof.
+  intros.
+  dup HINB1.
+  apply Ir.Memory.inbounds_blocks2_singleton2 in HINB0.
+  dup HINB2.
+  apply Ir.Memory.inbounds_blocks2_singleton2 in HINB3.
+  destruct l.
+  { eauto. }
+  destruct l.
+  { destruct l'. eauto.
+    destruct l'.
+    { destruct p. destruct p0.
+      destruct (b =? b0) eqn:HEQID.
+      { rewrite PeanoNat.Nat.eqb_eq in HEQID.
+        subst b0.
+        assert (List.In (b, t) (Ir.Memory.blocks m)).
+        { eapply Ir.Memory.inbounds_blocks2_In2.
+          rewrite HINB1. reflexivity. }
+        assert (List.In (b, t0) (Ir.Memory.blocks m)).
+        { eapply Ir.Memory.inbounds_blocks2_In2.
+          rewrite HINB2. reflexivity. }
+        eapply Ir.Memory.blocks_get in H; try eassumption; try reflexivity.
+        eapply Ir.Memory.blocks_get in H0; try eassumption; try reflexivity.
+        simpl in *. left. congruence. }
+      { rewrite PeanoNat.Nat.eqb_neq in HEQID.
+        dup HINB1.
+        dup HINB2.
+        eapply Ir.Memory.inbounds_blocks2_forallb2 in HINB4.
+        simpl in HINB4.
+        repeat (rewrite andb_true_r in HINB4).
+        eapply Ir.Memory.inbounds_blocks2_forallb2 in HINB5.
+        simpl in HINB5.
+        repeat (rewrite andb_true_r in HINB5).
+        (* make alive *)
+        dup HINB1.
+        apply Ir.Memory.inbounds_blocks2_alive in HINB6. simpl in HINB6.
+        rewrite andb_true_r in HINB6.
+        dup HINB2.
+        apply Ir.Memory.inbounds_blocks2_alive in HINB7. simpl in HINB7.
+        rewrite andb_true_r in HINB7.
+        (* inbounds_blocks2 -> List.In *)
+        symmetry in HINB1.
+        eapply Ir.Memory.inbounds_blocks2_In2 in HINB1.
+        symmetry in HINB2.
+        eapply Ir.Memory.inbounds_blocks2_In2 in HINB2.
+        rewrite andb_true_iff in HINB4. destruct HINB4.
+        rewrite andb_true_iff in H0. destruct H0.
+        rewrite andb_true_iff in HINB5. destruct HINB5.
+        rewrite andb_true_iff in H3. destruct H3.
+        dup HWF. inv HWF.
+        assert (disjoint_ranges (Ir.Memory.alive_P0_ranges m) = true).
+        { eapply disjoint_lsubseq_disjoint.
+          eapply wf_disjoint.
+          eapply Ir.Memory.alive_P_P0_ranges_lsubseq.
+          assumption. }
+        assert (disjoint_range (Ir.MemBlock.P0_range t)
+                               (Ir.MemBlock.P0_range t0) = true).
+        { eapply Ir.Memory.disjoint_range_P0_range.
+          eassumption.
+          apply In_get in HINB1; try assumption. eassumption.
+          assumption.
+          apply In_get in HINB2; try assumption. eassumption.
+          assumption.
+          assumption. }
+        (* okay, now let's get inconsistency. *)
+        unfold Ir.MemBlock.P0_range in H6.
+        simpl in H6.
+        unfold disjoint_range in H6.
+        rewrite orb_true_iff in H6.
+        rewrite PeanoNat.Nat.leb_le in H6.
+        rewrite PeanoNat.Nat.leb_le in H6.
+        unfold Ir.MemBlock.inbounds_abs in H, H0, H2, H3.
+        unfold in_range in H, H0, H2, H3.
+        rewrite andb_true_iff in H, H0, H2, H3.
+        unfold Ir.MemBlock.P0_range in H, H0, H2, H3.
+        simpl in H, H0, H2, H3.
+        repeat (rewrite PeanoNat.Nat.leb_le in *).
+        omega.
+      }
+    }
+    simpl in HINB3.
+    omega.
+  }
+  simpl in HINB0. omega.
+  assumption.
+  assumption.
+  assumption.
+  assumption.
+Qed.
+
+(* Very important lemma. *)
+Lemma physicalized_ptr_phy_I:
+  forall v1 v2 m
+         (HPP:physicalized_ptr m v1 v2),
+    forall md l1 o1 o2 I2 cid2 mb st
+         (HM:m = Ir.Config.m st)
+         (HWF:Ir.Config.wf md st)
+         (HV1:v1 = Ir.ptr (Ir.plog l1 o1))
+         (HV2:v2 = Ir.ptr (Ir.pphy o2 I2 cid2))
+         (HGET:Some mb = Ir.Memory.get (Ir.Config.m st) l1),
+    List.forallb (fun i => Ir.MemBlock.inbounds_abs i mb) I2 = true.
+Proof.
+  intros v1 v2 st HPP.
+  induction HPP.
+  { intros.
+    unfold Ir.ptr_to_phy in HP2.
+    destruct p1.
+    { unfold Ir.log_to_phy in HP2.
+      inv HV1.
+      rewrite <- HGET in HP2.
+      inv HP2.
+      inv HV2. reflexivity. }
+    { inv HP2. inv HV2. reflexivity. }
+  }
+  { intros.
+    inv HV1.
+    inv HV2.
+    unfold Ir.SmallStep.gep in H.
+    des_ifs.
+    { unfold Ir.SmallStep.gep in H1.
+      des_ifs.
+      { rewrite Heq in HGET. inv HGET. symmetry in Heq.
+        simpl.
+        dup HWF. inv HWF.
+        eapply physicalized_ptr_log in HPP; try eassumption; try reflexivity.
+        rewrite andb_true_iff in Heq0.
+        destruct Heq0.
+        rewrite <- HPP.
+        symmetry in Heq.
+        erewrite inbounds_abs_true with (n0 := n); try eassumption; try reflexivity.
+        erewrite inbounds_tcadd_abs; try eassumption; try reflexivity.
+        erewrite IHHPP; try reflexivity; try eassumption.
+        congruence.
+      }
+      { rewrite Heq in HGET. inv HGET. symmetry in Heq.
+        simpl.
+        dup HWF. inv HWF.
+        eapply physicalized_ptr_log in HPP; try eassumption; try reflexivity.
+        rewrite andb_true_iff in Heq0.
+        destruct Heq0.
+        rewrite <- HPP.
+        symmetry in Heq.
+        erewrite inbounds_abs_true with (n0 := n); try eassumption; try reflexivity.
+        erewrite inbounds_tcadd_abs; try eassumption; try reflexivity.
+        erewrite IHHPP; try reflexivity; try eassumption.
+        congruence.
+      }
+    }
+    { unfold Ir.SmallStep.gep in H1.
+      des_ifs.
+      erewrite IHHPP; try reflexivity; try eassumption.
+    }
+  }
+Qed.
+
+(* NOTE: This lemma does not hold anymore if function call is introduced.
+ This lemma should be replaced with something else which gives criteria
+ to cid. (ex: cid is never bogus) *)
+Lemma physicalized_ptr_phy_cid:
+  forall v1 v2 m
+         (HPP:physicalized_ptr m v1 v2),
+    forall md l1 o1 o2 I2 cid2 mb st
+         (HM:m = Ir.Config.m st)
+         (HWF:Ir.Config.wf md st)
+         (HV1:v1 = Ir.ptr (Ir.plog l1 o1))
+         (HV2:v2 = Ir.ptr (Ir.pphy o2 I2 cid2))
+         (HGET:Some mb = Ir.Memory.get (Ir.Config.m st) l1),
+      cid2 = None.
+Proof.
+  intros v1 v2 m HPP.
+  induction HPP.
+  { intros. inv HV1. inv HV2. unfold Ir.ptr_to_phy in HP2.
+    unfold Ir.log_to_phy in HP2.
+    des_ifs.
+  }
+  { intros. inv HV1. inv HV2.
+    unfold Ir.SmallStep.gep in *.
+    des_ifs.
+    { eapply IHHPP.
+      reflexivity. eassumption. reflexivity. reflexivity. eassumption. }
+    { eapply IHHPP.
+      reflexivity. eassumption. reflexivity. reflexivity. eassumption. }
+    { eapply IHHPP.
+      reflexivity. eassumption. reflexivity. reflexivity. eassumption. }
+  }
+Qed.
+
+Lemma mod_gt:
+  forall n m p (HP:p > 0), n mod p > m -> n > m.
+Proof.
+  intros.
+  unfold "mod" in H.
+  destruct p. inv H.
+  assert (p <= p). omega.
+  apply Nat.divmod_spec with (x := n) (q := 0) in H0.
+  destruct (Nat.divmod n p 0 p).
+  simpl in *.
+  destruct H0.
+  rewrite Nat.mul_0_r in *.
+  rewrite Nat.sub_diag in *.
+  rewrite Nat.add_0_r in *.
+  rewrite Nat.add_0_r in *.
+  rewrite H0.
+  eapply Nat.lt_le_trans.
+  eapply H.
+  apply le_plus_r.
+Qed.
+  
+
+Lemma mod_sub:
+  forall n m p (HN:n mod p >= m) (HP:p > 0),
+    (n mod p - m) = ((n - m) mod p).
+Proof.
+  admit.
+Admitted.
+
+Lemma get_deref_gep_pphy_inb_success:
+  forall m t p0 b t0 o I cid n0 idx sz
+    (HWF:Ir.Memory.wf m)
+    (HGET:Ir.Memory.get m b = Some t0)
+    (HSZ:sz > 0)
+    (HGEP:Ir.SmallStep.gep (Ir.pphy o I cid) idx t m true = Ir.ptr p0)
+    (HDEREF:Ir.get_deref m (Ir.pphy o I cid) sz = [(b, t0, n0)])
+    (HINB1:Ir.MemBlock.inbounds_abs ((o + idx * Ir.ty_bytesz t) mod Ir.MEMSZ)
+                                    t0 = true)
+    (HINB2:Ir.MemBlock.inbounds_abs ((o + idx * Ir.ty_bytesz t) mod Ir.MEMSZ + sz)
+                                    t0 = true),
+  Ir.get_deref m p0 sz =
+  [(b, t0, Ir.SmallStep.twos_compl_add n0 (idx * Ir.ty_bytesz t) Ir.PTRSZ)].
+Proof.
+  intros.
+  assert (HINB3:Ir.MemBlock.inbounds_abs o t0 = true).
+  { dup HDEREF.
+    apply Ir.get_deref_phy_singleton in HDEREF0; try assumption.
+    destruct HDEREF0; try congruence.
+    destruct H. destruct H. inv H. simpl in H0.
+    destruct H0.
+    apply Ir.get_deref_inv in HDEREF; try congruence.
+    rewrite andb_true_iff in HDEREF. destruct HDEREF.
+    rewrite andb_true_iff in H1. destruct H1.
+    erewrite Ir.MemBlock.inbounds_inbounds_abs in H3. eapply H3. omega. }
+  assert (HINB4:Ir.MemBlock.inbounds_abs (o+sz) t0 = true).
+  { dup HDEREF.
+    apply Ir.get_deref_phy_singleton in HDEREF0; try assumption.
+    destruct HDEREF0; try congruence.
+    destruct H. destruct H. inv H. simpl in H0.
+    destruct H0.
+    apply Ir.get_deref_inv in HDEREF; try congruence.
+    rewrite andb_true_iff in HDEREF. destruct HDEREF.
+    rewrite andb_true_iff in H1. destruct H1.
+    erewrite Ir.MemBlock.inbounds_inbounds_abs in H2. eapply H2. omega. }
+
+  unfold Ir.SmallStep.gep in HGEP.
+  des_ifs.
+  { (* positive offset *)
+    unfold Ir.get_deref in *.
+
+    assert (Ir.get_deref_blks_phyptr m
+       (Ir.SmallStep.twos_compl_add o (idx * Ir.ty_bytesz t) Ir.PTRSZ)
+       (o :: Ir.SmallStep.twos_compl_add o (idx * Ir.ty_bytesz t) Ir.PTRSZ :: I)
+       cid sz = (Ir.get_deref_blks_phyptr m o I cid sz)).
+    { admit. }
+    rewrite H.
+    remember (Ir.get_deref_blks_phyptr m o I cid sz) as res.
+    destruct res. simpl in HDEREF. inv HDEREF.
+    destruct res.
+    { simpl in HDEREF. inv HDEREF.
+      simpl.
+      assert (Ir.SmallStep.twos_compl_add o (idx * Ir.ty_bytesz t) Ir.PTRSZ -
+                                          Ir.MemBlock.addr (snd p) =
+              Ir.SmallStep.twos_compl_add (o - Ir.MemBlock.addr (snd p)) 
+                                          (idx * Ir.ty_bytesz t) Ir.PTRSZ).
+      { unfold Ir.SmallStep.twos_compl_add.
+        unfold Ir.SmallStep.twos_compl.
+        rewrite PTRSZ_MEMSZ.
+        rewrite mod_sub.
+        admit.
+        { unfold Ir.MemBlock.inbounds_abs in HINB1.
+          unfold in_range in HINB1.
+          unfold Ir.MemBlock.P0_range in HINB1.
+          simpl in HINB1.
+          rewrite andb_true_iff in HINB1.
+          destruct HINB1. rewrite Nat.leb_le in H0. omega. }
+        { assert (HH := MEMSZ_nonzero). omega. }
+      }
+      rewrite H0.
+      reflexivity.
+    }
+    { simpl in HDEREF. inv HDEREF. }
+  }
+  { (* negative offset *)
+    unfold Ir.get_deref in *.
+    assert (HPHYP:Ir.get_deref_blks_phyptr m
+       (Ir.SmallStep.twos_compl_add o (idx * Ir.ty_bytesz t) Ir.PTRSZ)
+       (o :: Ir.SmallStep.twos_compl_add o (idx * Ir.ty_bytesz t) Ir.PTRSZ :: I)
+       cid sz = (Ir.get_deref_blks_phyptr m o I cid sz)).
+    { admit. }
+    rewrite HPHYP.
+    destruct (Ir.get_deref_blks_phyptr m o I cid sz).
+    { simpl in HDEREF. inv HDEREF. }
+    destruct l.
+    { simpl in HDEREF. inv HDEREF.
+      simpl.
+      assert (Ir.SmallStep.twos_compl_add o (idx * Ir.ty_bytesz t) Ir.PTRSZ -
+              Ir.MemBlock.addr (snd p) =
+              Ir.SmallStep.twos_compl_add (o - Ir.MemBlock.addr (snd p)) 
+                                          (idx * Ir.ty_bytesz t) Ir.PTRSZ).
+      { unfold Ir.SmallStep.twos_compl_add.
+        unfold Ir.SmallStep.twos_compl.
+        rewrite PTRSZ_MEMSZ.
+        rewrite mod_sub.
+        admit.
+        { unfold Ir.MemBlock.inbounds_abs in HINB1.
+          unfold in_range in HINB1.
+          unfold Ir.MemBlock.P0_range in HINB1.
+          simpl in HINB1.
+          rewrite andb_true_iff in HINB1.
+          destruct HINB1. rewrite Nat.leb_le in H. omega. }
+        { assert (HH := MEMSZ_nonzero). omega. }
+      }
+      rewrite H. reflexivity.
+    }
+    simpl in HDEREF.
+    inv HDEREF.
+  }
+Admitted.
+
+Lemma get_deref_physicalized_ptr:
+  forall md st sz p1 p2
+         (HWF:Ir.Config.wf md st)
+         (HSZ:sz> 0)
+         (HPP:physicalized_ptr (Ir.Config.m st) (Ir.ptr p1) (Ir.ptr p2)),
+    (exists blk, Ir.get_deref (Ir.Config.m st) p1 sz = [blk] /\
+                 Ir.get_deref (Ir.Config.m st) p2 sz = [blk]) \/
+    (Ir.get_deref (Ir.Config.m st) p1 sz = []).
+Proof.
+  intros.
+  dup HWF.
+  inv HWF.
+  remember (Ir.ptr p1) as v1.
+  remember (Ir.ptr p2) as v2.
+  generalize dependent p1.
+  generalize dependent p2.
+  clear wf_cid_to_f.
+  clear wf_cid_to_f2.
+  clear wf_stack.
+  clear wf_no_bogus_ptr.
+  clear wf_no_bogus_ptr_mem.
+  remember (Ir.Config.m st) as m.
+  generalize dependent st.
+  induction HPP.
+  { intros.
+    rename p0 into p2'.
+    rename p3 into p1'.
+    inv Heqv2. inv Heqv1.
+    remember (Ir.Config.m st) as m.
+    remember (Ir.get_deref m p1' sz) as bb.
+    symmetry in Heqbb.
+    dup Heqbb.
+    apply Ir.get_deref_singleton in Heqbb0; try eauto.
+    destruct Heqbb0.
+    { destruct H. destruct H. inv H.
+      eapply Ir.get_deref_ptr_phy_same with (p' := p2') in H1;
+        try eauto.
+    }
+    { right. eauto. }
+  }
+  { intros.
+    assert (IHHPP' := IHHPP wf_m st Heqm HWF0
+                            p2 (eq_refl (Ir.ptr p2)) p1 (eq_refl (Ir.ptr p1))).
+    clear IHHPP.
+    destruct IHHPP'.
+    { (* exists deref p1. *)
+      destruct H.
+      destruct H.
+      inv Heqv2.
+      destruct p2.
+      { (* p2 is never log -> no *)
+        eapply physicalized_ptr_nonlog in HPP.
+        exfalso. eapply HPP. eauto. }
+      { destruct p1.
+        { (* log, pphy *)
+          destruct inb.
+          { (* inb *)
+            unfold Ir.SmallStep.gep in Heqv1.
+            des_ifs.
+            assert (HALIVE:Ir.MemBlock.alive t0 = true).
+            { unfold Ir.get_deref in H.
+              rewrite Heq in H. des_ifs.
+              rewrite andb_true_iff in Heq1.
+              destruct Heq1.
+              rewrite andb_true_iff in H.
+              destruct H.
+              assumption.
+            }
+            (* Now we have:
+               Given Ir.plog(b, n0), n0 was inbounds of t0 and
+               (n0 + idx * |ty|) % (2^PTRSZ) is also inboundos f t0. *)
+            (* Let's make: (int)(log(b, n0)) = n. *)
+            eapply physicalized_ptr_log with (mb := t0) in HPP;
+              try reflexivity; try congruence.
+            rewrite andb_true_iff in Heq0. destruct Heq0.
+            (* okay, n + idx * |ty| should be also inbounds_abs! *)
+            assert (Ir.MemBlock.inbounds_abs
+                      ((n + idx * (Ir.ty_bytesz t)) mod Ir.MEMSZ) t0 = true).
+            { eapply inbounds_added_abs_true; try eassumption. }
+            (* n should be inbounds_abs as well. *)
+            assert (Ir.MemBlock.inbounds_abs n t0 = true).
+            { eapply inbounds_abs_true; try eassumption. }
+            (* Is n + idx*|t| + sz inbounds? *)
+            destruct (Ir.MemBlock.inbounds
+                        (Ir.SmallStep.twos_compl_add n0
+                          (idx * Ir.ty_bytesz t) Ir.PTRSZ + sz) t0) eqn:HINB.
+            { (* yes, inbounds. *)
+              (* n + idx*|t| + sz should be inbounds_abs as well. *)
+              assert (Ir.MemBlock.inbounds_abs
+                        ((n + (idx * (Ir.ty_bytesz t))) mod Ir.MEMSZ + sz) t0 = true).
+              { eapply inbounds_added_abs_true2; try eassumption. }
+              (*, okay now get get_deref m (r.plog b (n0 + idx * |t|)). *)
+              dup H.
+              eapply Ir.get_deref_log in H7; try eassumption.
+              destruct H7; try congruence.
+              inv H7.
+              assert (Ir.get_deref (Ir.Config.m st) (Ir.plog b
+                (Ir.SmallStep.twos_compl_add n0 (idx * Ir.ty_bytesz t) Ir.PTRSZ)) sz =
+                [(b, t0,
+                  (Ir.SmallStep.twos_compl_add n0 (idx * Ir.ty_bytesz t) Ir.PTRSZ))]).
+              { unfold Ir.get_deref.
+                rewrite Heq.
+                rewrite HALIVE.
+                rewrite HINB.
+                rewrite H3.
+                reflexivity. }
+              left.
+              eexists.
+              split. eassumption.
+              eapply get_deref_gep_pphy_inb_success; try eassumption.
+            }
+            { (* no, ofs+sz is not inbounds. cannot deref *)
+              right.
+              unfold Ir.get_deref.
+              rewrite Heq.
+              rewrite HINB.
+              rewrite andb_false_r. reflexivity. }
+          }
+          { (* inb = false *)
+            admit.
+          }
+        }
+        { (* pphy and pphy. *)
+          admit.
+        }
+      }
+    }
+    { (* deref p1 failed. *)
+      destruct p2.
+      { (* p2 is never log -> no *)
+        eapply physicalized_ptr_nonlog in HPP.
+        exfalso. eapply HPP. eauto. }
+      { destruct p1.
+        { (* p1 is log. *)
+          unfold Ir.get_deref in H.
+          des_ifs.
+          { (* IR.Memory.get b makes sense *)
+            clear Heq0.
+            (* make condition on I *)
+            dup HPP.
+            eapply physicalized_ptr_phy_I in HPP0; try eassumption;
+              try reflexivity.
+            2: rewrite Heq. 2: reflexivity.
+            (* make condition on cid. *)
+            dup HPP.
+            eapply physicalized_ptr_phy_cid in HPP; try eassumption; try reflexivity.
+            2: rewrite Heq. 2: reflexivity.
+            subst o.
+            (* what is gep (plog)? *)
+            unfold Ir.SmallStep.gep in Heqv1.
+            des_ifs.
+            { (* inbounds *)
+              remember (Ir.get_deref (Ir.Config.m st)
+                (Ir.plog b (Ir.SmallStep.twos_compl_add n0 
+                            (idx * Ir.ty_bytesz t) Ir.PTRSZ)) sz) as blks.
+              symmetry in Heqblks.
+              
+            dup Heqblks.
+            eapply Ir.get_deref_log_s
+      
+     
+
+
 
 Lemma get_deref_physicalized_ptr:
   forall md st sz p1 p2
@@ -312,7 +1225,7 @@ Proof.
     { (* p1 was log. *)
       destruct inb eqn:HINB.
       { (* inbounds *)
-        des_ifs.
+(*        des_ifs.
         (* okay, how about p2? *)
         unfold Ir.SmallStep.gep in Heqv2.
         destruct p2.
@@ -326,6 +1239,11 @@ Proof.
             2: rewrite Heq.
             2: reflexivity.
             (* okay, Ir.plog b n and Ir.pphy (n0 l o) has same integer repr. *)
+            dup HPP.
+            apply physicalized_ptr_log with (mb := t0) (l1 := b) (o1 := n)
+              (o2 := n0) (Is2 := l) (cid2 := o) in HPP0;
+              try congruence.
+            
             
             assert (Ir.get_deref m (Ir.plog b n) sz = [(b, t0, n)]).
             { unfold Ir.get_deref.
@@ -335,8 +1253,10 @@ Proof.
               destruct (Ir.MemBlock.alive t0).
               { simpl. 
           { (* added offset was negative - no check *)
-    
-    
+  *) admit.
+      }
+      { inv Heqv1.
+        
     
 
 Theorem load_refines:
